Code/Preprocessing/Error.v
@@ -1,0 +1,66 @@
+Require Import Basics.
+Require Import List.
+
+Declare Scope error.
+
+Inductive error (A : Type) : Type :=
+| Ret : A -> error A
+| TypeCheckErrorNoVar : error A
+| TypeCheckErrorNoBase : error A
+| TypeCheckErrorOther : error A
+| ScopeError : error A
+| UndefinedSymbol : error A.
+
+Arguments Ret {_} _.
+Arguments TypeCheckErrorNoVar {_}.
+Arguments TypeCheckErrorNoBase {_}.
+Arguments TypeCheckErrorOther {_}.
+Arguments ScopeError {_}.
+Arguments UndefinedSymbol {_}.
+
+Definition error_return
+           (A : Type)
+  : A -> error A
+  := Ret.
+
+Definition error_map
+           {A B : Type}
+           (f : A -> B)
+           (x : error A)
+  : error B
+  := match x with
+     | Ret a => Ret (f a)
+     | TypeCheckErrorNoVar => TypeCheckErrorNoVar
+     | TypeCheckErrorNoBase => TypeCheckErrorNoBase
+     | TypeCheckErrorOther => TypeCheckErrorOther
+     | ScopeError => ScopeError
+     | UndefinedSymbol => UndefinedSymbol
+     end.
+
+Definition error_bind
+           {A B : Type}
+           (x : error A)
+           (f : A -> error B)
+  : error B
+  := match x with
+     | Ret a => f a
+     | TypeCheckErrorNoVar => TypeCheckErrorNoVar
+     | TypeCheckErrorNoBase => TypeCheckErrorNoBase
+     | TypeCheckErrorOther => TypeCheckErrorOther
+     | ScopeError => ScopeError
+     | UndefinedSymbol => UndefinedSymbol
+     end.
+
+Notation "x >>= f" := (error_bind x f) : error.
+
+Local Open Scope error.
+
+Fixpoint list_error
+         {A : Type}
+         (l : list (error A))
+  : error (list A)
+  := match l with
+     | nil => Ret nil
+     | x :: xs =>
+       list_error xs >>= fun ys => x >>= fun y => Ret (y :: ys)
+     end.
